src/Pipit.System.fst
@@ -186,3 +186,71 @@ let rec step0_ok
     let hBS' = bigstep_substitute_XMu e1 streams [v] hBS in
     let (| s1', () |) = step0_ok e1 (v :: row) v hBS' in
     (| explicit_cast (state_of_exp e) s1', () |)
+
+#push-options "--split_queries"
+let rec stepn_ok
+  (#outer: nat { outer > 0 }) (#vars: nat)
+  (e: exp { causal e /\ wf e vars })
+  (row: C.row vars)
+  (streams: C.table outer vars)
+  (v: value)
+  (vs: C.vector value outer)
+  (hBS: bigstep (C.table_append (C.table1 row) streams) e (v :: vs))
+  (s: state_of_exp e)
+  (u: unit { system_of_exp_invariant #(outer - 1) e streams vs (bigstep_monotone #outer hBS) s }):
+    Tot (s': state_of_exp e & u: unit { system_of_exp e vars (C.row_elts row) (Some s) s' v /\ system_of_exp_invariant #outer e (C.table_append (C.table1 row) streams) (v :: vs) hBS s' }) (decreases e) =
+  let streams' = C.table_append (C.table1 row) streams in
+  match e with
+  | XVal _ -> (| (), () |)
+  | XVar x -> (| (), () |)
+
+  | XPrim2 p e1 e2 ->
+    let BSPrim2 _ _ _ _ (v1 :: vs1) (v2 :: vs2) hBS1 hBS2 = hBS in
+    let (s1, s2) = s <: (state_of_exp e1 * state_of_exp e2) in
+    let (| s1', () |) = stepn_ok e1 row streams v1 vs1 hBS1 s1 () in
+    let (| s2', () |) = stepn_ok e2 row streams v2 vs2 hBS2 s2 () in
+    (| (s1', s2'), () |)
+
+  | XPre e1 ->
+    let BSPre _ _ _ (vx :: vs1) hBS1 = hBS in
+    let (s1, v1) = s <: (state_of_exp e1 * value) in
+    let v1' = bigstep_monotone_inv_next #outer #vars #streams' hBS1 in
+    let hBS1' = bigstep_monotone_inv #outer #vars #streams' hBS1 in
+
+    bigstep_proof_equivalence (bigstep_monotone_inv (bigstep_monotone #(outer - 1) hBS1)) hBS1;
+    bigstep_proof_equivalence hBS1 (bigstep_monotone #outer hBS1');
+    let (| s1', () |) = stepn_ok e1 row streams v1' (v1 :: vs1) hBS1' s1 () in
+    (| (s1', v1'), () |)
+
+  | XThen e1 e2 ->
+    let BSThen _ _ _ (v1 :: vs1) (v2 :: vs2) hBS1 hBS2 = hBS in
+    let s2 = explicit_cast (state_of_exp e2) s in
+    // let (| s1', () |) = stepn_ok e1 row streams v1 vs1 hBS1 s1 () in
+    let (| s2', () |) = stepn_ok e2 row streams v2 vs2 hBS2 s2 () in
+    (| explicit_cast (state_of_exp e) s2', () |)
+
+
+  | XMu e1 ->
+    let hBS' = bigstep_substitute_XMu e1 streams' (v :: vs) hBS in
+    let s1 = explicit_cast (state_of_exp e1) s in
+    bigstep_proof_equivalence (bigstep_substitute_XMu e1 streams vs (bigstep_monotone #outer hBS)) (bigstep_monotone #outer (bigstep_substitute_XMu e1 streams' (v :: vs) hBS));
+    let (| s1', () |) = stepn_ok e1 (C.row_append (C.row1 v) row) (C.table_map_append (C.table_of_values vs) streams) v vs hBS' s1 () in
+    (| explicit_cast (state_of_exp e) s1', () |)
+
+
+let rec step_many_ok
+  (#outer: nat { outer > 0 }) (#vars: nat)
+  (e: exp { causal e /\ wf e vars })
+  (streams: C.table outer vars)
+  (vs: C.vector value outer)
+  (hBS: bigstep streams e vs):
+    Tot (s': state_of_exp e & u: unit { system_of_exp_invariant #(outer - 1) e streams vs hBS s' }) (decreases outer) =
+  match streams, vs with
+  | C.Table [C.Row row], [v] ->
+    let (| s, () |) = step0_ok e row v hBS in
+    (| s, () |)
+
+  | C.Table (r :: rs'), v :: vs' ->
+    let (| s, () |) = step_many_ok e (C.Table #(outer - 1) rs') vs' (bigstep_monotone #(outer - 1) hBS) in
+    let (| s', () |) = stepn_ok #(outer - 1) e r (C.Table #(outer - 1) rs') v vs' hBS s () in
+    (| s', () |)
